src/Narcissus/Formats/FixListOpt.v
@@ -74,12 +74,12 @@ Section FixList.
   Proof.
     split.
     {
-      intros env env' xenv l l' ext ? Eeq Ppred Ppred_rest Penc.
+      intros env env' xenv l ext ? Eeq Ppred Ppred_rest Penc.
       intuition; subst.
       revert H0.
       generalize dependent env. generalize dependent env'.
       generalize dependent xenv.
-      generalize dependent l'. induction l.
+      generalize dependent bin. induction l.
       { intros.
         simpl in *; intuition; computes_to_inv;
           injections; simpl.
@@ -89,7 +89,7 @@ Section FixList.
         unfold Bind2 in Penc; computes_to_inv; subst.
         destruct v; destruct v0; simpl in *.
         injections.
-        destruct (fun H' => proj1 A_decode_pf _ _ _ _ _ (mappend b0 ext) env_OK Eeq H H' Penc) as [ ? [? [? xenv_OK] ] ].
+        destruct (fun H' => proj1 (A_decode_pf _) _ _ _ _ (mappend b0 ext) env_OK Eeq H H' Penc) as [ ? [? [? xenv_OK] ] ].
         intuition; destruct_ex.
         eapply H1; eauto.
         setoid_rewrite <- mappend_assoc; setoid_rewrite H1;
@@ -99,14 +99,14 @@ Section FixList.
         eexists; intuition.
       }
     }
-    { induction sz; simpl; intros.
+    { generalize dependent bin. induction sz; simpl; intros.
       - injections; simpl; repeat eexists; intuition eauto.
         symmetry; apply mempty_left.
       - destruct (A_decode bin env') as [ [ [? ?] ?] | ] eqn: ? ;
           simpl in *; try discriminate.
         destruct (decode_list sz b c) as [ [ [? ?] ?] | ] eqn: ? ;
           simpl in *; try discriminate; injections.
-        eapply (proj2 A_decode_pf) in Heqo; eauto;
+        eapply (proj2 (A_decode_pf _)) in Heqo; eauto;
           destruct Heqo; destruct_ex; intuition; subst;
             eapply IHsz in Heqo0; eauto; destruct Heqo0;
               destruct_ex; intuition; subst.
